Simpler nonexpansiveness proofs for funspecs.

mailbox/acq_rel_atomics.v
@@ -7,6 +7,8 @@ Require Import mailbox.general_atomics.
 
 Set Bullet Behavior "Strict Subproofs".
 
+(* Invariants are probably unsound under RA. How can we prove linearizability of RA programs, then? *)
+
 Definition gsh1 := fst (Share.split Tsh).
 Definition gsh2 := snd (Share.split Tsh).
 
@@ -28,51 +30,51 @@ Qed.
 Section atomics.
 
 Context {CS : compspecs}.
-Context {state : Type} `{state_ord : PCM_order state}.
-Variable (s0 : state).
-
-(* Iris-weak gives a more in-depth encoding of protocol assertions in terms of invariants and ghost state. This
-   simpler one is probably still sound and almost as powerful. *)
-Definition protocol_inv T l g g' := EX v : Z, EX s : state, !!(field_compatible tint [] l /\ repable_signed v) &&
-  mapsto Tsh tint l (vint v) * ghost_master s g * ghost_var gsh1 s g' * T s v.
-
-Definition protocol_R l g g' (s : state) T := invariant (protocol_inv T l g g') * ghost_snap s g.
-
-Definition protocol_W l g g' (s : state) T := invariant (protocol_inv T l g g') * ghost_var gsh2 s g'.
-
-Lemma protocol_inv_super_non_expansive : forall n T l g g',
-  compcert_rmaps.RML.R.approx n (protocol_inv T l g g') =
-  compcert_rmaps.RML.R.approx n (protocol_inv (fun s v => compcert_rmaps.RML.R.approx n (T s v)) l g g').
-Proof.
-  intros; unfold protocol_inv.
-  rewrite !approx_exp; apply f_equal; extensionality v.
-  rewrite !approx_exp; apply f_equal; extensionality s.
-  rewrite !approx_sepcon, !approx_andp, approx_idem; auto.
-Qed.
-
-Lemma protocol_R_super_non_expansive : forall n l g g' s T,
-  compcert_rmaps.RML.R.approx n (protocol_R l g g' s T) =
-  compcert_rmaps.RML.R.approx n (protocol_R l g g' s (fun s v => compcert_rmaps.RML.R.approx n (T s v))).
-Proof.
-  intros; unfold protocol_R.
-  rewrite !approx_sepcon; f_equal.
-  rewrite invariant_super_non_expansive; setoid_rewrite invariant_super_non_expansive at 2.
-  rewrite protocol_inv_super_non_expansive; auto.
-Qed.
-
-Lemma protocol_W_super_non_expansive : forall n l g g' s T,
-  compcert_rmaps.RML.R.approx n (protocol_W l g g' s T) =
-  compcert_rmaps.RML.R.approx n (protocol_W l g g' s (fun s v => compcert_rmaps.RML.R.approx n (T s v))).
-Proof.
-  intros; unfold protocol_W.
-  rewrite !approx_sepcon; f_equal.
-  rewrite invariant_super_non_expansive; setoid_rewrite invariant_super_non_expansive at 2.
-  rewrite protocol_inv_super_non_expansive; auto.
-Qed.
-
-(* Can we also open general invariants at an atomic, since they won't involve the current values of RA locations? *)
 
 Definition duplicable P := view_shift P (P * P).
+
+Lemma emp_duplicable : duplicable emp.
+Proof.
+  repeat intro.
+  rewrite sepcon_emp in H; auto.
+Qed.
+Hint Resolve emp_duplicable : dup.
+
+Lemma sepcon_duplicable : forall P Q, duplicable P -> duplicable Q -> duplicable (P * Q).
+Proof.
+  intros; unfold duplicable.
+  rewrite <- sepcon_assoc, (sepcon_comm (_ * Q)), <- sepcon_assoc, sepcon_assoc.
+  apply view_shift_sepcon; auto.
+Qed.
+Hint Resolve sepcon_duplicable : dup.
+
+Lemma sepcon_list_duplicable : forall lP, Forall duplicable lP -> duplicable (fold_right sepcon emp lP).
+Proof.
+  induction 1; simpl; auto with dup.
+Qed.
+
+Lemma invariant_duplicable : forall P, duplicable (invariant P).
+Proof.
+  intros; unfold duplicable; rewrite invariant_duplicable at 1; reflexivity.
+Qed.
+Hint Resolve invariant_duplicable : dup.
+
+Lemma ghost_snap_duplicable : forall `{_ : PCM_order} (s : A) p, duplicable (ghost_snap s p).
+Proof.
+  intros; unfold duplicable.
+  erewrite ghost_snap_join; [reflexivity|].
+  apply ord_join; reflexivity.
+Qed.
+Hint Resolve ghost_snap_duplicable : dup.
+
+Lemma prop_duplicable : forall P Q, duplicable Q -> duplicable (!!P && Q).
+Proof.
+  intros.
+  apply view_shift_prop; intro.
+  etransitivity; eauto.
+  apply derives_view_shift; entailer!.
+Qed.
+Hint Resolve prop_duplicable : dup.
 
 Lemma duplicable_super_non_expansive : forall n P, compcert_rmaps.RML.R.approx n (!!duplicable P) =
   compcert_rmaps.RML.R.approx n (!!duplicable (compcert_rmaps.RML.R.approx n P)).
@@ -81,184 +83,181 @@ Proof.
   rewrite view_shift_super_non_expansive, approx_sepcon; auto.
 Qed.
 
-Definition LA_type := ProdType (ProdType (ProdType (ConstType (val * val * val * state))
-  (ArrowType (ConstType state) (ArrowType (ConstType Z) Mpred))) Mpred) (ArrowType (ConstType Z) Mpred).
+Section protocols.
+
+Context {state : Type}.
+
+(* Iris-weak gives a more in-depth encoding of protocol assertions in terms of invariants and ghost state. This
+   simpler one is probably still sound and almost as powerful. *)
+Definition protocol_inv (ord : state -> state -> Prop) T l g g' := EX v : Z, EX s : state,
+  !!(field_compatible tint [] l /\ repable_signed v) &&
+  mapsto Tsh tint l (vint v) * ghost_master s g * ghost_var gsh1 s g' * T s v.
+
+Definition protocol_R l g g' (s : state) ord T := invariant (protocol_inv ord T l g g') * ghost_snap s g.
+
+Definition protocol_W l g g' (s : state) ord T := invariant (protocol_inv ord T l g g') * ghost_var gsh2 s g'.
+
+Lemma protocol_inv_super_non_expansive : forall n ord T l g g',
+  compcert_rmaps.RML.R.approx n (protocol_inv ord T l g g') =
+  compcert_rmaps.RML.R.approx n (protocol_inv ord (fun s v => compcert_rmaps.RML.R.approx n (T s v)) l g g').
+Proof.
+  intros; unfold protocol_inv.
+  rewrite !approx_exp; apply f_equal; extensionality v.
+  rewrite !approx_exp; apply f_equal; extensionality s.
+  rewrite !approx_sepcon, !approx_andp, approx_idem; auto.
+Qed.
+
+Lemma protocol_R_super_non_expansive : forall n l g g' s ord T,
+  compcert_rmaps.RML.R.approx n (protocol_R l g g' s ord T) =
+  compcert_rmaps.RML.R.approx n (protocol_R l g g' s ord (fun s v => compcert_rmaps.RML.R.approx n (T s v))).
+Proof.
+  intros; unfold protocol_R.
+  rewrite !approx_sepcon; f_equal.
+  rewrite invariant_super_non_expansive; setoid_rewrite invariant_super_non_expansive at 2.
+  rewrite protocol_inv_super_non_expansive; auto.
+Qed.
+
+Lemma protocol_W_super_non_expansive : forall n l g g' s ord T,
+  compcert_rmaps.RML.R.approx n (protocol_W l g g' s ord T) =
+  compcert_rmaps.RML.R.approx n (protocol_W l g g' s ord (fun s v => compcert_rmaps.RML.R.approx n (T s v))).
+Proof.
+  intros; unfold protocol_W.
+  rewrite !approx_sepcon; f_equal.
+  rewrite invariant_super_non_expansive; setoid_rewrite invariant_super_non_expansive at 2.
+  rewrite protocol_inv_super_non_expansive; auto.
+Qed.
+
+Context `{PCM_order state}.
+
+Lemma protocol_R_duplicable : forall l g g' s ord T, duplicable (protocol_R l g g' s ord T).
+Proof.
+  intros; unfold protocol_R.
+  apply sepcon_duplicable; auto with dup.
+  apply ghost_snap_duplicable.
+Qed.
+
+End protocols.
+
+Definition OrdType s := ArrowType s (ArrowType s (ConstType Prop)).
+
+Definition LA_type := ProdType (ProdType (ProdType (ProdType (ProdType (ConstType (val * val * val))
+  (DependentType 0)) (OrdType (DependentType 0)))
+  (ArrowType (DependentType 0) (ArrowType (ConstType Z) Mpred))) Mpred) (ArrowType (ConstType Z) Mpred).
 
 Program Definition load_acq_spec := TYPE LA_type
-  WITH l : val, g : val, g' : val, s : state, T : state -> Z -> mpred, P : mpred, Q : Z -> mpred
+  WITH l : val, g : val, g' : val, s : _, ord : _ -> _ -> Prop, T : _ -> Z -> mpred, P : mpred, Q : Z -> mpred
   PRE [ 1%positive OF tptr tint ]
    PROP (forall s' v, ord s s' -> repable_signed v -> view_shift (P * T s' v) (Q v); forall v, duplicable (Q v))
    LOCAL (temp 1%positive l)
-   SEP (protocol_R l g g' s T; P)
+   SEP (protocol_R l g g' s ord T; P)
   POST [ tint ]
-   EX v : Z, EX s' : state,
+   EX v : Z, EX s' : _,
    PROP (repable_signed v; ord s s')
    LOCAL (temp ret_temp (vint v))
-   SEP (protocol_R l g g' s' T; Q v).
+   SEP (protocol_R l g g' s' ord T; Q v).
 Next Obligation.
 Proof.
-  replace _ with (fun (_ : list Type) (x : _) rho =>
-    PROP (let '(l, g, g', s, T, P, Q) := x in (forall s' v, ord s s' -> repable_signed v ->
-      view_shift (P * T s' v) (Q v)) /\ forall v, duplicable (Q v))
-    LOCAL (let '(l, g, g', s, T, P, Q) := x in temp 1%positive l)
-    SEP (let '(l, g, g', s, T, P, Q) := x in protocol_R l g g' s T * P) rho).
-  apply (PROP_LOCAL_SEP_super_non_expansive LA_type [fun _ => _] [fun _ => _] [fun _ => _]);
-    repeat constructor; hnf; intros; destruct x as ((((((?, ?), ?), ?), ?), ?), ?); auto; simpl.
+  repeat intro.
+  destruct x as (((((((?, ?), ?), s), ?), ?), ?), ?); simpl.
+  unfold PROPx; simpl; rewrite !approx_andp; f_equal.
   - rewrite !prop_and, !approx_andp; f_equal.
-    + rewrite !prop_forall, !(approx_allp _ _ _ s0); f_equal; extensionality s'.
+    + rewrite !prop_forall, !(approx_allp _ _ _ s); f_equal; extensionality s'.
       rewrite !prop_forall, !(approx_allp _ _ _ 0); f_equal; extensionality v'.
       rewrite !prop_impl; setoid_rewrite approx_imp; do 2 apply f_equal.
       setoid_rewrite approx_imp; do 2 apply f_equal.
       rewrite view_shift_super_non_expansive, !approx_sepcon; auto.
-    + rewrite !prop_forall, !(approx_allp _ _ _ 0); f_equal; extensionality v'.
+    + f_equal.
+      rewrite !prop_forall, !(approx_allp _ _ _ 0); f_equal; extensionality v'.
       apply duplicable_super_non_expansive.
-  - rewrite !approx_sepcon, protocol_R_super_non_expansive, approx_idem; auto.
-  - extensionality ts x rho.
-    destruct x as ((((((?, ?), ?), ?), ?), ?), Q); simpl.
-    unfold PROPx, SEPx; simpl; rewrite !sepcon_assoc, !and_assoc; auto.
+  - unfold LOCALx; simpl; rewrite !approx_andp; apply f_equal.
+    unfold SEPx; simpl; rewrite !approx_sepcon, protocol_R_super_non_expansive, approx_idem; auto.
 Qed.
 Next Obligation.
 Proof.
-  replace _ with (fun (_ : list Type) (x : _ * mpred * _) rho =>
-    EX v : Z, EX s' : state,
-      PROP (let '(l, g, g', s, T, P, Q) := x in repable_signed v /\ ord s s')
-      LOCAL (let '(l, g, g', s, T, P, Q) := x in temp ret_temp (vint v))
-      SEP (let '(l, g, g', s, T, P, Q) := x in protocol_R l g g' s' T * Q v) rho).
-  - repeat intro.
-    rewrite !approx_exp; apply f_equal; extensionality v.
-    rewrite !approx_exp; apply f_equal; extensionality s'.
-    apply (PROP_LOCAL_SEP_super_non_expansive LA_type [fun _ '(l, g, g', s, T, P, Q) => _]
-      [fun _ '(l, g, g', s, T, P, Q) => _] [fun _ '(l, g, g', s, T, P, Q) => _]);
-      repeat constructor; hnf; intros; destruct x0 as ((((((?, ?), ?), ?), ?), ?), ?); auto; simpl.
-    rewrite !approx_sepcon, protocol_R_super_non_expansive, approx_idem; auto.
-  - extensionality ts x rho.
-    destruct x as ((((((?, ?), ?), ?), ?), ?), ?); simpl.
-    apply f_equal; extensionality.
-    apply f_equal; extensionality.
-    unfold PROPx, SEPx; simpl; rewrite !sepcon_assoc, !and_assoc; auto.
+  repeat intro.
+  destruct x as (((((((?, ?), ?), ?), ?), ?), ?), ?); simpl.
+  rewrite !approx_exp; apply f_equal; extensionality vr.
+  rewrite !approx_exp; apply f_equal; extensionality s'.
+  unfold PROPx; simpl; rewrite !approx_andp; apply f_equal.
+  unfold LOCALx; simpl; rewrite !approx_andp; apply f_equal.
+  unfold SEPx; simpl; rewrite !approx_sepcon, protocol_R_super_non_expansive, approx_idem; auto.
 Qed.
 
-Definition SR_type := ProdType (ProdType (ProdType (ConstType (val * Z * val * val * state * state))
-  (ArrowType (ConstType state) (ArrowType (ConstType Z) Mpred))) Mpred) Mpred.
-
-Notation "'TYPE' A 'WITH'  x1 : t1 , x2 : t2 , x3 : t3 , x4 : t4 , x5 : t5 , x6 : t6 , x7 : t7 , x8 : t8 , x9 : t9 'PRE'  [ u , .. , v ] P 'POST' [ tz ] Q" :=
-     (mk_funspec ((cons u%formals .. (cons v%formals nil) ..), tz) cc_default A
-  (fun (ts: list Type) (x: t1*t2*t3*t4*t5*t6*t7*t8*t9) =>
-     match x with (x1,x2,x3,x4,x5,x6,x7,x8,x9) => P%assert end)
-  (fun (ts: list Type) (x: t1*t2*t3*t4*t5*t6*t7*t8*t9) =>
-     match x with (x1,x2,x3,x4,x5,x6,x7,x8,x9) => Q%assert end) _ _)
-            (at level 200, x1 at level 0, x2 at level 0, x3 at level 0, x4 at level 0,
-             x5 at level 0, x6 at level 0, x7 at level 0, x8 at level 0, x9 at level 0,
-             P at level 100, Q at level 100).
+Definition SR_type := ProdType (ProdType (ProdType (ProdType (ProdType (ProdType (ConstType (val * Z * val * val))
+  (DependentType 0)) (DependentType 0)) (OrdType (DependentType 0)))
+  (ArrowType (DependentType 0) (ArrowType (ConstType Z) Mpred))) Mpred) Mpred.
 
 Program Definition store_rel_spec := TYPE SR_type
-  WITH l : val, v : Z, g : val, g' : val, s : state, s'' : state, T : state -> Z -> mpred, P : mpred, Q : mpred
+  WITH l : val, v : Z, g : val, g' : val, s : _, s'' : _, st_ord : _ -> _ -> Prop, T : _ -> Z -> mpred, P : mpred, Q : mpred
   PRE [ 1%positive OF tptr tint, 2%positive OF tint ]
-   PROP (repable_signed v; forall v0, repable_signed v0 -> view_shift (P * T s v0) (T s'' v * Q); ord s s'')
+   PROP (repable_signed v; forall v0, repable_signed v0 -> view_shift (P * T s v0) (T s'' v * Q); st_ord s s'')
    LOCAL (temp 1%positive l; temp 2%positive (vint v))
-   SEP (protocol_W l g g' s T; P)
+   SEP (protocol_W l g g' s st_ord T; P)
   POST [ tvoid ]
    PROP ()
    LOCAL ()
-   SEP (protocol_W l g g' s'' T; Q).
+   SEP (protocol_W l g g' s'' st_ord T; Q).
 Next Obligation.
 Proof.
-  replace _ with (fun (_ : list Type) (x : _) rho =>
-    PROP (let '(l, v, g, g', s, s'', T, P, Q) := x in repable_signed v /\ (forall v0, repable_signed v0 ->
-      view_shift (P * T s v0) (T s'' v * Q)) /\ ord s s'')
-    LOCAL (let '(l, v, g, g', s, s'', T, P, Q) := x in temp 1%positive l;
-           let '(l, v, g, g', s, s'', T, P, Q) := x in temp 2%positive (vint v))
-    SEP (let '(l, v, g, g', s, s'', T, P, Q) := x in protocol_W l g g' s T * P) rho).
-  apply (PROP_LOCAL_SEP_super_non_expansive SR_type [fun _ => _] [fun _ => _; fun _ => _] [fun _ => _]);
-    repeat constructor; hnf; intros; destruct x as ((((((((?, ?), ?), ?), ?), ?), ?), ?), ?); auto; simpl.
+  repeat intro.
+  destruct x as (((((((((?, ?), ?), ?), ?), ?), ?), ?), ?), ?); simpl.
+  unfold PROPx; simpl; rewrite !approx_andp; f_equal.
   - rewrite !prop_and, !approx_andp; f_equal; f_equal.
     rewrite !prop_forall, !(approx_allp _ _ _ 0); f_equal; extensionality v'.
     rewrite !prop_impl; setoid_rewrite approx_imp; do 2 apply f_equal.
     rewrite view_shift_super_non_expansive, !approx_sepcon; auto.
-  - rewrite !approx_sepcon, protocol_W_super_non_expansive, approx_idem; auto.
-  - extensionality ts x rho.
-    destruct x as ((((((((?, ?), ?), ?), ?), ?), ?), ?), ?); simpl.
-    unfold PROPx, SEPx; simpl; rewrite !sepcon_assoc, !and_assoc; auto.
+  - unfold LOCALx; simpl; rewrite !approx_andp; apply f_equal.
+    unfold SEPx; simpl; rewrite !approx_sepcon, protocol_W_super_non_expansive, approx_idem; auto.
 Qed.
 Next Obligation.
 Proof.
-  replace _ with (fun (_ : list Type) (x : _ * Z * _ * _ * state * _ * _ * mpred * _) rho =>
-    PROP ()
-    LOCAL ()
-    SEP (let '(l, v, g, g', s, s'', T, P, Q) := x in protocol_W l g g' s'' T * Q) rho).
-  - repeat intro.
-    apply (PROP_LOCAL_SEP_super_non_expansive SR_type [] [] [fun _ '(l, v, g, g', s, s'', T, P, Q) => _]);
-      repeat constructor; hnf; intros; destruct x0 as ((((((((?, ?), ?), ?), ?), ?), ?), ?), ?); auto; simpl.
-    rewrite !approx_sepcon, protocol_W_super_non_expansive, approx_idem; auto.
-  - extensionality ts x rho.
-    destruct x as ((((((((?, ?), ?), ?), ?), ?), ?), ?), ?); simpl.
-    unfold SEPx; simpl; rewrite !sepcon_assoc; auto.
+  repeat intro.
+  destruct x as (((((((((?, ?), ?), ?), ?), ?), ?), ?), ?), ?); simpl.
+  unfold PROPx; simpl; rewrite !approx_andp; apply f_equal.
+  unfold LOCALx; simpl; rewrite !approx_andp; apply f_equal.
+  unfold SEPx; simpl; rewrite !approx_sepcon, protocol_W_super_non_expansive, approx_idem; auto.
 Qed.
 
-Definition CRA_type := ProdType (ProdType (ProdType (ConstType (val * Z * Z * val * val * state * state))
-  (ArrowType (ConstType state) (ArrowType (ConstType Z) Mpred))) Mpred) (ArrowType (ConstType Z) Mpred).
-
-Notation "'TYPE' A 'WITH'  x1 : t1 , x2 : t2 , x3 : t3 , x4 : t4 , x5 : t5 , x6 : t6 , x7 : t7 , x8 : t8 , x9 : t9 , x10 : t10 'PRE'  [ u , .. , v ] P 'POST' [ tz ] Q" :=
-     (mk_funspec ((cons u%formals .. (cons v%formals nil) ..), tz) cc_default A
-  (fun (ts: list Type) (x: t1*t2*t3*t4*t5*t6*t7*t8*t9*t10) =>
-     match x with (x1,x2,x3,x4,x5,x6,x7,x8,x9,x10) => P%assert end)
-  (fun (ts: list Type) (x: t1*t2*t3*t4*t5*t6*t7*t8*t9*t10) =>
-     match x with (x1,x2,x3,x4,x5,x6,x7,x8,x9,x10) => Q%assert end) _ _)
-            (at level 200, x1 at level 0, x2 at level 0, x3 at level 0, x4 at level 0,
-             x5 at level 0, x6 at level 0, x7 at level 0, x8 at level 0, x9 at level 0, x10 at level 0,
-             P at level 100, Q at level 100).
+Definition CRA_type := ProdType (ProdType (ProdType (ProdType (ProdType (ProdType (ConstType (val * Z * Z * val * val))
+  (DependentType 0)) (DependentType 0)) (OrdType (DependentType 0)))
+  (ArrowType (DependentType 0) (ArrowType (ConstType Z) Mpred))) Mpred) (ArrowType (ConstType Z) Mpred).
 
 Program Definition CAS_RA_spec := TYPE CRA_type
-  WITH l : val, c : Z, v : Z, g : val, g' : val, s : state, s'' : state, T : state -> Z -> mpred, P : mpred, Q : Z -> mpred
+  WITH l : val, c : Z, v : Z, g : val, g' : val, s : _, s'' : _, ord : _ -> _ -> Prop, T : _ -> Z -> mpred,
+       P : mpred, Q : Z -> mpred
   PRE [ 1%positive OF tptr tint, 2%positive OF tint, 3%positive OF tint ]
    PROP (repable_signed c; repable_signed v; forall v0, repable_signed v0 ->
      view_shift (P * T s v0) ((if eq_dec v0 c then T s'' v else T s v0) * Q v0); ord s s'')
    LOCAL (temp 1%positive l; temp 2%positive (vint c); temp 3%positive (vint v))
-   SEP (protocol_W l g g' s T; P)
+   SEP (protocol_W l g g' s ord T; P)
   POST [ tint ]
    EX v' : Z,
    PROP (repable_signed v')
    LOCAL (temp ret_temp (Val.of_bool (if eq_dec v' c then true else false)))
-   SEP (protocol_W l g g' (if eq_dec v' c then s'' else s) T; Q v').
+   SEP (protocol_W l g g' (if eq_dec v' c then s'' else s) ord T; Q v').
 Next Obligation.
 Proof.
-  replace _ with (fun (_ : list Type) (x : _) rho =>
-    PROP (let '(l, c, v, g, g', s, s'', T, P, Q) := x in repable_signed c /\ repable_signed v /\
-          (forall v0, repable_signed v0 -> view_shift (P * T s v0) ((if eq_dec v0 c then T s'' v else T s v0) * Q v0))
-          /\ ord s s'')
-    LOCAL (let '(l, c, v, g, g', s, s'', T, P, Q) := x in temp 1%positive l;
-           let '(l, c, v, g, g', s, s'', T, P, Q) := x in temp 2%positive (vint c);
-           let '(l, c, v, g, g', s, s'', T, P, Q) := x in temp 3%positive (vint v))
-    SEP (let '(l, c, v, g, g', s, s'', T, P, Q) := x in protocol_W l g g' s T * P) rho).
-  apply (PROP_LOCAL_SEP_super_non_expansive CRA_type [fun _ => _] [fun _ => _; fun _ => _; fun _ => _] [fun _ => _]);
-    repeat constructor; hnf; intros; destruct x as (((((((((?, ?), ?), ?), ?), ?), ?), ?), ?), ?); auto; simpl.
+  repeat intro.
+  destruct x as ((((((((((?, ?), ?), ?), ?), ?), ?), ?), ?), ?), ?); simpl.
+  unfold PROPx; simpl; rewrite !approx_andp; f_equal.
   - rewrite !prop_and, !approx_andp; do 2 apply f_equal; f_equal.
     rewrite !prop_forall, !(approx_allp _ _ _ 0); f_equal; extensionality v'.
     rewrite !prop_impl; setoid_rewrite approx_imp; do 2 apply f_equal.
     rewrite view_shift_super_non_expansive, !approx_sepcon; if_tac; auto.
-  - rewrite !approx_sepcon, protocol_W_super_non_expansive, approx_idem; auto.
-  - extensionality ts x rho.
-    destruct x as (((((((((?, ?), ?), ?), ?), ?), ?), ?), ?), ?); simpl.
-    unfold PROPx, SEPx; simpl; rewrite !sepcon_assoc, !and_assoc; auto.
+  - unfold LOCALx; simpl; rewrite !approx_andp; f_equal.
+    unfold SEPx; simpl.
+    rewrite !approx_sepcon, protocol_W_super_non_expansive, approx_idem; auto.
 Qed.
 Next Obligation.
 Proof.
-  replace _ with (fun (_ : list Type) (x : _ * _ * Z * _ * _ * _ * _ * _ * mpred * _) rho =>
-    EX v' : Z,
-      PROP (let '(l, c, v, g, g', s, s'', T, P, Q) := x in repable_signed v')
-      LOCAL (let '(l, c, v, g, g', s, s'', T, P, Q) := x in temp ret_temp (Val.of_bool (if eq_dec v' c then true else false)))
-      SEP (let '(l, c, v, g, g', s, s'', T, P, Q) := x in protocol_W l g g' (if eq_dec v' c then s'' else s) T *
-           Q v') rho).
-  - repeat intro.
-    rewrite !approx_exp; apply f_equal; extensionality v'.
-    apply (PROP_LOCAL_SEP_super_non_expansive CRA_type [fun _ '(l, c, v, g, g', s, s'', T, P, Q) => _]
-      [fun _ '(l, c, v, g, g', s, s'', T, P, Q) => _] [fun _ '(l, c, v, g, g', s, s'', T, P, Q) => _]);
-      repeat constructor; hnf; intros; destruct x0 as (((((((((?, ?), ?), ?), ?), ?), ?), ?), ?), ?); auto; simpl.
-    rewrite !approx_sepcon, protocol_W_super_non_expansive, approx_idem; auto.
-  - extensionality ts x rho.
-    destruct x as (((((((((?, ?), ?), ?), ?), ?), ?), ?), ?), ?); simpl.
-    apply f_equal; extensionality.
-    unfold SEPx; simpl; rewrite !sepcon_assoc; auto.
+  repeat intro.
+  destruct x as ((((((((((?, ?), ?), ?), ?), ?), ?), ?), ?), ?), ?); simpl.
+  rewrite !approx_exp; apply f_equal; extensionality vr.
+  unfold PROPx; simpl; rewrite !approx_andp; f_equal.
+  unfold LOCALx; simpl; rewrite !approx_andp; f_equal.
+  unfold SEPx; simpl; rewrite !approx_sepcon, protocol_W_super_non_expansive, approx_idem; auto.
 Qed.
 
 End atomics.
+
+Hint Resolve emp_duplicable sepcon_duplicable invariant_duplicable ghost_snap_duplicable prop_duplicable : dup.
